src/rocq/Semantics/Memory/MemoryBytes.v
@@ -12,9 +12,6 @@ From Vellvm Require Import
   DynamicTypes
   VellvmIntegers
   Utils.ErrUbOomProp
-  Utils.Oomable
-  Utils.Poisonable
-  Utils.ErrOomPoison
   Utils.ListUtil
   Syntax.LLVMAst
   Memory.Sizeof.
@@ -99,7 +96,7 @@ Fixpoint concat_bytes_Z (bytes : list Z) : Z
          byte + (Z.shiftl (concat_bytes_Z bytes) 8)
      end.
 
-Module Type DvalueByte (LP : LLVMParams).
+Module Type MemoryByte (LP : LLVMParams).
   Import LP.
   Import PTOI.
   Import ITOP.
@@ -137,12 +134,9 @@ Module Type DvalueByte (LP : LLVMParams).
    *)
 (*  Obligation Tactic := try Tactics.program_simpl; try solve [cbn; try lia | solve_dvalue_measure]. *)
 
-  Variant DByte : Type := | DBPoison | DBV (n : Z).
-  Notation dbv n := (ret (DBV n)).
-
   (* offset is the number of bytes indexed past so far *)
   Fixpoint dvalue_extract_byte
-    {M} `{Monad M} `{RAISE_ERROR M} `{RAISE_OOMABLE M}
+    {M} `{Monad M} `{RAISE_ERROR M}
     (dv : dvalue) (dt : dtyp) (idx : Z) {struct dv} : eitherT string M Z :=
     let dvalue_extract_struct_bytes (pad : option N) : list dvalue -> list dtyp -> N -> Z -> eitherT string M Z :=
       fix loop fields types (offset : N) (idx : Z) {struct fields} : eitherT string M Z :=
@@ -219,7 +213,6 @@ Module Type DvalueByte (LP : LLVMParams).
        | DVALUE_Double d =>
            ret (extract_byte_Z (unsigned (Float.to_bits d)) idx)
        | DVALUE_Poison dt => raise "Extracting poison byte"
-       | DVALUE_Oom dt => raise_oomable dt
        | DVALUE_None =>
            (* TODO: Not sure if this should be an error, poison, or what. *)
            raise_error "dvalue_extract_byte on DVALUE_None"
@@ -259,19 +252,19 @@ Module Type DvalueByte (LP : LLVMParams).
 
       Unlike UVALUE_ExtractByte, I don't think this needs an sid
       (store id). There should be no nondeterminism in this value. *)
-  Inductive dvalue_byte : Type :=
-  | DVALUE_ExtractByte (dv : dvalue) (dt : dtyp) (idx : N) : dvalue_byte
+  Inductive memory_byte : Type :=
+  | MByte (dv : dvalue) (dt : dtyp) (idx : N) : memory_byte
   .
 
-  Definition dvalue_byte_value {M} `{Monad M} `{RAISE_ERROR M} `{RAISE_OOMABLE M} (db : dvalue_byte) : eitherT string M Z 
+  Definition memory_byte_value {M} `{Monad M} `{RAISE_ERROR M} (db : memory_byte) : eitherT string M Z 
     := match db with
-       | DVALUE_ExtractByte dv dt idx =>
+       | MByte dv dt idx =>
            dvalue_extract_byte dv dt (Z.of_N idx)
        end.
 
-  Definition dvalue_to_dvalue_bytes (dv : dvalue) (dt : dtyp) : list dvalue_byte
+  Definition dvalue_to_memory_bytes (dv : dvalue) (dt : dtyp) : list memory_byte
     := map
-         (fun idx => (DVALUE_ExtractByte dv dt idx))
+         (fun idx => (MByte dv dt idx))
          (Nseq 0 (N.to_nat (sizeof_dtyp dt))).
 
   #[local] Obligation Tactic := try Tactics.program_simpl; try solve [cbn; try lia].
@@ -287,9 +280,14 @@ Module Type DvalueByte (LP : LLVMParams).
                                | inr v => k v
                                end). 
   
-  Fixpoint dvalue_bytes_to_dvalue {M} {HM: Monad M} {HRM: RAISE_ERROR M} {HOM: RAISE_OOMABLE M} (dbs : list dvalue_byte) (dt : dtyp) : M dvalue :=
-
-    let list_dvalue_bytes_to_dvalue (pad : option N) :=
+  Definition dtyp_is_void (dt : dtyp) : bool := match dt with | DTYPE_Void => true | _ => false end.
+  
+  Fixpoint memory_bytes_to_dvalue
+    {M} {HM: Monad M} {HRM: RAISE_ERROR M} {HOM: RAISE_OOM M} (dbs : list memory_byte) (dt : dtyp) : M dvalue :=
+    if dtyp_is_void dt
+    then raise_error "deserialize_sbytes: Attempt to deserialize void."%string
+    else
+    let list_memory_bytes_to_dvalue (pad : option N) :=
       fix go (offset : N) dts dbs :=
         match dts with
         | [] =>
@@ -309,7 +307,7 @@ Module Type DvalueByte (LP : LLVMParams).
             let init_bytes := take sz dbs' in
             let rest_bytes := drop sz dbs' in
             let offset' := offset + padding in
-            f <- dvalue_bytes_to_dvalue init_bytes dt ;;
+            f <- memory_bytes_to_dvalue init_bytes dt ;;
             rest <- go (offset' + sz) dts rest_bytes ;;
             ret (f :: rest)
         end
@@ -318,53 +316,55 @@ Module Type DvalueByte (LP : LLVMParams).
     match dt with
     | DTYPE_I sz =>
         bind_down_cast dt
-          (map_monad (dvalue_byte_value) dbs)
+          (map_monad (memory_byte_value) dbs)
           (fun v => ret (@DVALUE_I sz (concat_bytes_Z_vint v)))
    
     | DTYPE_IPTR =>
         bind_down_cast dt
-        (map_monad dvalue_byte_value dbs)
+        (map_monad memory_byte_value dbs)
         (fun zs : list Z =>
-         bind (lift_OOMABLE DTYPE_IPTR (IP.from_Z (concat_bytes_Z zs)))
-           (fun val : IP.intptr => ret (DVALUE_IPTR val)))
+           match IP.from_Z (concat_bytes_Z zs) with
+           | NoOom val => ret (DVALUE_IPTR val)
+           | Oom s => raise_oom s
+           end) 
 
     | DTYPE_Pointer =>
         (* TODO: not sure if this should be wildcard provenance.
                 TODO: not sure if this should truncate iptr value...
          *)
         (* TODO: not sure if this should be lazy OOM or not *)
-        bind_down_cast dt (map_monad dvalue_byte_value dbs)
+        bind_down_cast dt (map_monad memory_byte_value dbs)
           (fun zs => match int_to_ptr (concat_bytes_Z zs) wildcard_prov with
                   | NoOom a => ret (DVALUE_Addr a)
-                  | Oom msg => raise_oomable DTYPE_Pointer
+                  | Oom msg => raise_oom "TODO: Not sure if this should be lazy oom or not?"
                   end)
             
     | DTYPE_Void =>
-        raise_error "dvalue_bytes_to_dvalue on void type."
+        raise_error "memory_bytes_to_dvalue on void type."
     | DTYPE_FP FP_half =>
-        raise_error "dvalue_bytes_to_dvalue: unsupported half."
+        raise_error "memory_bytes_to_dvalue: unsupported half."
     | DTYPE_FP FP_bfloat =>
-        raise_error "dvalue_bytes_to_dvalue: unsupported bfloat"
+        raise_error "memory_bytes_to_dvalue: unsupported bfloat"
     | DTYPE_FP FP_float =>
-        bind_down_cast dt (map_monad dvalue_byte_value dbs)
+        bind_down_cast dt (map_monad memory_byte_value dbs)
           (fun zs => ret (DVALUE_Float (Float32.of_bits (concat_bytes_Z_vint zs))))
     | DTYPE_FP FP_double => 
-        bind_down_cast dt (map_monad dvalue_byte_value dbs)
+        bind_down_cast dt (map_monad memory_byte_value dbs)
           (fun zs => ret (DVALUE_Double (Float.of_bits (concat_bytes_Z_vint zs))))
     | DTYPE_FP FP_x86_fp80 =>
-        raise_error "dvalue_bytes_to_dvalue: unsupported X86_fp80."
+        raise_error "memory_bytes_to_dvalue: unsupported X86_fp80."
     | DTYPE_FP FP_fp128 =>
-        raise_error "dvalue_bytes_to_dvalue: unsupported fp128."
+        raise_error "memory_bytes_to_dvalue: unsupported fp128."
     | DTYPE_FP FP_ppc_fp128 =>
-        raise_error "dvalue_bytes_to_dvalue: unsupported ppc_fp128."
+        raise_error "memory_bytes_to_dvalue: unsupported ppc_fp128."
     | DTYPE_Label =>
-        raise_error "dvalue_bytes_to_dvalue: unsupported DTYPE_Label."
+        raise_error "memory_bytes_to_dvalue: unsupported DTYPE_Label."
     | DTYPE_Token =>
-        raise_error "dvalue_bytes_to_dvalue: unsupported DTYPE_Token."
+        raise_error "memory_bytes_to_dvalue: unsupported DTYPE_Token."
     | DTYPE_Metadata =>
-        raise_error "dvalue_bytes_to_dvalue: unsupported DTYPE_Metadata."
+        raise_error "memory_bytes_to_dvalue: unsupported DTYPE_Metadata."
     | DTYPE_X86_mmx =>
-        raise_error "dvalue_bytes_to_dvalue: unsupported DTYPE_X86_mmx."
+        raise_error "memory_bytes_to_dvalue: unsupported DTYPE_X86_mmx."
     | DTYPE_Array sz t =>
         let sz' := sizeof_dtyp t in
         let elt_bytes :=
@@ -372,7 +372,7 @@ Module Type DvalueByte (LP : LLVMParams).
           then repeatN sz []
           else split_every_nil sz' dbs
         in
-        elts <- map_monad (fun es => dvalue_bytes_to_dvalue es t) elt_bytes;;
+        elts <- map_monad (fun es => memory_bytes_to_dvalue es t) elt_bytes;;
         ret (DVALUE_Array t elts)
     | DTYPE_Vector sz t =>
         let sz' := sizeof_dtyp t in
@@ -381,19 +381,19 @@ Module Type DvalueByte (LP : LLVMParams).
           then repeatN sz []
           else split_every_nil sz' dbs
         in
-        elts <- map_monad (fun es => dvalue_bytes_to_dvalue es t) elt_bytes;;
+        elts <- map_monad (fun es => memory_bytes_to_dvalue es t) elt_bytes;;
         ret (DVALUE_Vector t elts)
     | DTYPE_Struct fields =>
-        Functor.fmap DVALUE_Struct (list_dvalue_bytes_to_dvalue (Some (max_preferred_dtyp_alignment fields)) 0 fields dbs)
+        Functor.fmap DVALUE_Struct (list_memory_bytes_to_dvalue (Some (max_preferred_dtyp_alignment fields)) 0 fields dbs)
                      
     | DTYPE_Packed_struct fields =>
-        Functor.fmap DVALUE_Packed_struct (list_dvalue_bytes_to_dvalue None 0 fields dbs)
+        Functor.fmap DVALUE_Packed_struct (list_memory_bytes_to_dvalue None 0 fields dbs)
     | DTYPE_Opaque =>
-        raise_error "dvalue_bytes_to_dvalue: unsupported DTYPE_Opaque."
+        raise_error "memory_bytes_to_dvalue: unsupported DTYPE_Opaque."
     end.
 
-End DvalueByte.
+End MemoryByte.
 
-Module Make (LP : LLVMParams) <: DvalueByte LP.
-  Include (DvalueByte LP).
+Module Make (LP : LLVMParams) <: MemoryByte LP.
+  Include (MemoryByte LP).
 End Make.
