src/rocq/Semantics/StoreId.v
@@ -1,3 +1,0 @@
-From Stdlib Require Import ZArith.
-
-Definition store_id := N.
