src/rocq/Semantics/MemoryParams.v
@@ -1,20 +1,14 @@
 From Vellvm Require Import
      Semantics.LLVMParams
      Semantics.GepM
-     Semantics.Memory.MemBytes
-     Semantics.Memory.DvalueBytes.
+     Semantics.Memory.MemoryBytes.
 
 Module Type MEMORY_PARAMS (LP : LLVMParams).
   Declare Module GEP : GEPM LP.
-  Declare Module BYTE_IMPL : ByteImpl LP.
-  Declare Module DVALUE_BYTES : DvalueByte LP.
+  Declare Module MBYTES : MemoryByte LP.
 End MEMORY_PARAMS.
 
-Module Make (LP : LLVMParams) (GEP' : GEPM LP) (BYTE_IMPL' : ByteImpl LP) (DVALUE_BYTES' : DvalueByte LP) : MEMORY_PARAMS LP
-with Module GEP := GEP'
-with Module BYTE_IMPL := BYTE_IMPL'
-with Module DVALUE_BYTES := DVALUE_BYTES'.
-  Module GEP := GEP'.
-  Module BYTE_IMPL := BYTE_IMPL'.
-  Module DVALUE_BYTES := DVALUE_BYTES'.
+Module Make (LP : LLVMParams) : MEMORY_PARAMS LP.
+  Module GEP := GepM.Make LP.
+  Module MBYTES := MemoryBytes.Make LP.
 End Make.
